- Defined a notions of refinement of methods of an ADT, which allows changing the [Model].
- Defined a notion of refinement of an entire ADT, using above notions of refinement.

- Updated TODO

- Makefile now includes ADTRefinement.

ADTRefinement.v
@@ -43,26 +43,139 @@ Section pick.
   
 End pick.
 
+Section MethodRefinement.
+
+  Variables (oldModel newModel : Type). (* Old and new model *)
+  Variable absNewModel : newModel -> oldModel -> Prop.  
+  (* Abstraction relation from new to old models *)
+  
+  Variable abs : newModel -> oldModel. (* Abstraction function *)
+  Variable absValid : forall nm, absNewModel nm (abs nm). 
+
+  (* Refinement of an observer method *)
+  Definition refineObserver 
+             (newObserver : observerMethodType newModel) 
+             (oldObserver : observerMethodType oldModel) :=
+      forall nm om n, 
+        absNewModel nm om -> 
+        refine (oldObserver om n) (newObserver nm n).
+  
+  (* Refinement of a mutator method *)
+  Definition refineMutator 
+             (newMutator : mutatorMethodType newModel)
+             (oldMutator : mutatorMethodType oldModel) :=
+    forall nm om n, 
+      absNewModel nm om -> 
+      forall nm', 
+        computes_to (newMutator nm n) nm' -> (* For any new mutated state *)
+          computes_to (oldMutator om n) (abs nm'). 
+  
+End MethodRefinement.
+
 Inductive refineADT : ADT -> ADT -> Prop := 
-  | refinesADT : 
-      forall oldModel newModel 
-             (*  Relationship between old and new (at least as concrete) model *)
-             (RepInv : oldModel -> newModel -> Prop) 
-             mutatorMethodIndex observerMethodIndex
-             (* Assumes indices are the same, we alternatively establish 
-              that there is an injection from old indices to new indices. *)
-             (oldMutatorMethods : mutatorMethodIndex -> mutatorMethodType oldModel)
-             (newMutatorMethods : mutatorMethodIndex -> mutatorMethodType newModel)
-             (oldObserverMethods : observerMethodIndex -> observerMethodType oldModel)
-             (newObserverMethods : observerMethodIndex -> observerMethodType newModel),
-        (* Need to specify that each mutator is a refinement 
-           This should correspond to lifting [RepInv] to [Comp].
-        (forall idx om nm n a, 
-           RepInv om nm -> 
-           refine (newMutatorMethods idx nm n) (oldMutatorMethods idx om n)) -> *)
-        (* Each observer is a refinement *)
-        (forall idx om nm n, 
-           RepInv om nm -> 
-           refine (newObserverMethods idx nm n) (oldObserverMethods idx om n)) -> 
-        refineADT (Build_ADT newMutatorMethods newObserverMethods)
-                  (Build_ADT oldMutatorMethods oldObserverMethods).
+| refinesADT : 
+    forall (oldModel newModel : Type)
+           (absNewModel : newModel -> oldModel -> Prop)
+           (abs : newModel -> oldModel) (* Abstraction function *)
+           (absValid : forall nm, absNewModel nm (abs nm)) (* absNewModel is left-total *)
+           (oldObserverMethodIndex : Type) (* Old Observer Method Index Type *)
+           (newObserverMethodIndex : Type) (* New Observer Method Index Type 
+                                             (In order to add new observers) *)
+           (mapObserverIndex : oldObserverMethodIndex -> newObserverMethodIndex)
+           (* Map from old indices to new ones *)
+           (oldMutatorMethodIndex : Type) (* Old Mutator Method Index Type *)
+           (newMutatorMethodIndex : Type) (* New Mutator Method Index Type 
+                                           (In order to add new mutators) *)
+           (mapMutatorIndex : oldMutatorMethodIndex -> newMutatorMethodIndex)
+           (* Map from old indices to new ones *)
+           (oldObserverMethods : oldObserverMethodIndex -> observerMethodType oldModel)
+           (newObserverMethods : newObserverMethodIndex -> observerMethodType newModel)
+           (oldMutatorMethods : oldMutatorMethodIndex -> mutatorMethodType oldModel)
+           (newMutatorMethods : newMutatorMethodIndex -> mutatorMethodType newModel),
+      (forall idx idx', mapObserverIndex idx = mapObserverIndex idx' -> idx = idx') -> (* mapObserverIndex is injective *)
+      (forall idx idx', mapMutatorIndex idx = mapMutatorIndex idx' -> idx = idx') -> (* mapObserverIndex is injective *)
+      (forall idx, refineObserver absNewModel (newObserverMethods (mapObserverIndex idx)) (oldObserverMethods idx)) -> 
+      (forall idx, refineMutator absNewModel abs (newMutatorMethods (mapMutatorIndex idx)) (oldMutatorMethods idx)) -> 
+      refineADT (Build_ADT newMutatorMethods newObserverMethods)
+                (Build_ADT oldMutatorMethods oldObserverMethods).
+
+Theorem refineADT_inv old new :
+  refineADT new old -> 
+  match old with 
+    | {| Model := m;
+         MutatorIndex := mdx;
+         ObserverIndex := odx;
+         MutatorMethods := mutators;
+         ObserverMethods := observers |} => 
+      exists (absNewModel : Model new -> m -> Prop)
+             (abs : Model new -> m)
+             (mapObserverIndex : odx -> ObserverIndex new)
+             (mapMutatorIndex : mdx -> MutatorIndex new),
+        (forall nm, absNewModel nm (abs nm)) /\
+        (forall idx idx', mapObserverIndex idx = mapObserverIndex idx' -> idx = idx') /\
+      (forall idx idx', mapMutatorIndex idx = mapMutatorIndex idx' -> idx = idx') /\
+        (forall idx, refineObserver absNewModel (ObserverMethods new (mapObserverIndex idx)) (observers idx)) /\
+        (forall idx, refineMutator absNewModel abs (MutatorMethods new (mapMutatorIndex idx)) (mutators idx))
+        
+  end.
+Proof.
+  destruct 1; simpl; eauto 10.
+Qed.
+
+Section MethodPreOrders.
+
+  Variables (oldModel newModel : Type). (* Old and new model *)
+  Variable absNewModel : newModel -> oldModel -> Prop.  
+  Variable abs : newModel -> oldModel.
+  Variable absValid : forall nm, absNewModel nm (abs nm).
+  Variable observerMethodIndex : Type. (* Observer Method Index Type *)
+  Variable mutatorMethodIndex : Type. (* Mutator Method Index Type *)
+  Variable oldObserverMethods : observerMethodIndex -> observerMethodType oldModel.
+  Variable newObserverMethods : observerMethodIndex -> observerMethodType newModel.
+  Variable oldMutatorMethods : mutatorMethodIndex -> mutatorMethodType oldModel.
+  Variable newMutatorMethods : mutatorMethodIndex -> mutatorMethodType newModel.
+
+  Global Instance refineObserver_PreOrder Model : 
+    PreOrder (refineObserver (@eq Model)).
+  Proof.
+    split; compute in *; intros; subst; eauto.
+  Qed.
+
+  Add Parametric Relation Model : _ (refineObserver (@eq Model)) 
+      reflexivity proved by reflexivity
+      transitivity proved by transitivity
+    as refineObserver_rel.
+
+  Global Instance refineMutator_PreOrder Model : 
+    PreOrder (refineMutator (@eq Model) id).
+  Proof.
+    split; compute in *; intros; subst; eauto.
+  Qed.
+
+  Add Parametric Relation Model : _ (refineObserver (@eq Model)) 
+      reflexivity proved by reflexivity
+      transitivity proved by transitivity
+    as refineMutator_rel.
+
+  Global Instance refineADT_PreOrder
+  : PreOrder refineADT.
+  Proof.
+    split; compute in *.
+    intros; destruct x; econstructor 1 with 
+                        (absNewModel := @eq _)
+                          (mapObserverIndex := id)
+                          (mapMutatorIndex := id)
+                          (abs := id); eauto; reflexivity.
+    intros x y z Rxy Ryz; destruct Rxy.    
+    destruct z; inversion_by refineADT_inv.
+    compute in *.
+    econstructor 1 with (absNewModel := fun x' z => x (abs0 x') z)
+                          (mapMutatorIndex := compose mapMutatorIndex x2)
+                          (mapObserverIndex := compose mapObserverIndex x1)
+                          (abs := compose x0 abs0); 
+      eauto; compute in *; eauto.
+  Qed.
+
+End comp.
+
+Hint Constructors computes_to
